\documentclass[t,usenames,dvipsnames]{beamer}
\usetheme{Copenhagen}
\setbeamertemplate{headline}{} % remove toc from headers
\beamertemplatenavigationsymbolsempty

\usepackage{amsmath, xcolor, tikz, pgfplots}

\pgfplotsset{compat = 1.16}
\usetikzlibrary{arrows.meta, calc, decorations.pathreplacing}
\pgfplotsset{every axis/.append style = {axis lines = middle}}
\pgfplotsset{every tick label/.append style={font=\scriptsize}}
\everymath{\displaystyle}

\title{Graphs of Quadratic Expressions}
\author{}
\date{}

\AtBeginSection[]
{
  \begin{frame}
    \frametitle{Objectives}
    \tableofcontents[currentsection]
  \end{frame}
}

\begin{document}

\begin{frame}
    \maketitle
\end{frame}

\section{Determine the vertex and axis of symmetry of a quadratic function in standard form}

\begin{frame}{Graphing Quadratic Expressions}
We will be looking at graphing equations in the form
\[ y = ax^2 + bx + c \]
where $a$, $b$, and $c$ are real numbers with $a \neq 0$. 
\end{frame}

\begin{frame}{Graph of a Quadratic Expression}
For $y= x^2$, the graph below is a \alert{parabola}.
\begin{center}
\begin{tikzpicture}[scale=0.8]
\begin{axis}[
xmin = -3.5, xmax = 3.5,
ymin = -0.5, ymax = 4.75,
xtick = {-3,-2,...,3},
ytick = {1,2,3,4}
]
\addplot[color=blue, very thick, samples=200, smooth] {x^2};
\addplot[color=blue, mark=*, only marks] coordinates {(-2,4) (-1,1) (0,0) (1,1) (2,4)};
\node at (axis cs:-2,4) [left] {$(-2,4)$};
\node at (axis cs:-1,1) [left] {$(-1,1)$};
\node at (axis cs:0,0) [below] {$(0,0)$};
\node at (axis cs:1,1) [right] {$(1,1)$};
\node at (axis cs:2,4) [right] {$(2,4)$};
\end{axis}
\end{tikzpicture}
\end{center}
\end{frame}

\begin{frame}{Graph of a Quadratic Expression}
The point $(0,0)$ is called the \alert{vertex} of the parabola and can be either a minimum (smile) or maximum point (frown). \newline\\  \pause

Through the vertex is a vertical line called the \alert{axis of symmetry} that divides the parabola into 2 equal halves. 
\end{frame}

\begin{frame}{Example 1}
Find the vertex, state whether the vertex is a maximum or minimum, and find the equation of the axis of symmetry for each.   \newline\\
(a) \quad $y = x^2 + 4x + 1$  \newline\\
\begin{minipage}{0.6\textwidth}
\onslide<2->{
\begin{tikzpicture}[scale=0.8]
\begin{axis}[
xmin = -5, xmax = 1,
ymin = -4, ymax = 2,
xtick = {-4,-3,-2,-1,0},
ytick = {-3,-2,-1,0,1}
]
\addplot[color=blue, very thick, samples=200, smooth] {(x+2)^2 - 3};
\only<5->{\draw[color=red, dashed, very thick, <->, >=stealth] (axis cs: -2,-4) -- (axis cs: -2,2);}
\end{axis}
\end{tikzpicture} }
\end{minipage}
\hspace{-0.5cm}
\begin{minipage}{0.4\textwidth}
\onslide<3->{Vertex $(-2,-3)$}	\\[8pt]
\onslide<4->{Vertex is a minimum}	\\[8pt]
\onslide<5->{Axis of symmetry: $x = -2$}
\end{minipage}
\end{frame}


\begin{frame}{Example 1}
(b) \quad $y = -2x^2+12x-17$    \newline\\
\begin{minipage}{0.55\textwidth}
\onslide<2->{
\begin{tikzpicture}[scale=0.8]
\begin{axis}[
xmin = -1, xmax = 7,
ymin = -8, ymax = 2,
xtick = {-1,0,...,5},
ytick = {-7,-6,...,1}
]
\addplot[color=blue, very thick, samples=200, smooth, domain=0:6] {-2*(x-3)^2 + 1};
\only<5->{\draw[color=red, dashed, very thick, <->, >=stealth] (axis cs: 3,-8) -- (axis cs: 3,2);}
\end{axis}
\end{tikzpicture}}
\end{minipage}
\hspace{-0.25cm}
\begin{minipage}{0.4\textwidth}
\onslide<3->{Vertex $(3,1)$} \\[8pt]
\onslide<4->{Vertex is a maximum} \\[8pt]
\onslide<5->{Axis of symmetry: $x=3$}
\end{minipage}
\end{frame}


\section{Convert between standard and general form of quadratic expressions}

\begin{frame}{Standard and General Form of Quadratic Expressions}
For a quadratic function: \newline\\  
\begin{itemize}
    \item<+-> The \alert{general form} is $y = ax^2+bx+c$
    \begin{itemize}
        \item<+-> $a$, $b$, and $c$ are real numbers
        \item<+-> $a \neq 0$    
    \end{itemize}   \vspace{8pt}
    \item<+-> The \alert{standard form} is $y = a(x-h)^2 + k$
    \begin{itemize}
        \item<+-> Vertex is $(h,k)$
        \item<+-> $a \neq 0$
        \item<+-> $a$, $h$, and $k$ are real numbers
    \end{itemize}
\end{itemize}
\end{frame}

\begin{frame}{Converting From General to Standard Form}
    To convert from general form $y = ax^2 + bx + c$ to standard form $y = a(x-h)^2+k$ \newline\\
    \begin{enumerate}
        \onslide<2->{\item Find the vertex:}  \\[8pt]
        \begin{itemize}
            \onslide<2->{\item $x$-coordinate: $\frac{-b}{2a}$} \\[8pt]
            \onslide<2->{\item $y$-coordinate: Evaluate expression at $x$-coordinate} \\[8pt]
            \onslide<2->{\item Or use graphing technology} \\[8pt]
        \end{itemize}
        \onslide<2->{\item Use the same value of $a$}
    \end{enumerate}
\end{frame}

\begin{frame}{Example 2}
Convert each to standard form.  \newline\\
(a) \quad $y = x^2 - 4x + 3$ \newline\\
\onslide<2->{Vertex:} \newline\\
\onslide<3->{$x = \frac{-(-4)}{2(1)}$} \newline\\
\onslide<4->{$x = 2$} \newline\\
\onslide<5->{$y = 2^2 - 4(2) + 3$} \newline\\
\onslide<6->{$y = -1$}
\end{frame}

\begin{frame}{Example 2}
(a) \quad $y = x^2 - 4x + 3$ \newline\\
Vertex: $(2,-1)$    \newline\\
\onslide<2->{$a = 1$}
\onslide<3->{\[y = (x-2)^2 - 1\]}
\end{frame}

\begin{frame}{Example 2}
Convert each to standard form.  \newline\\
(b) \quad $y = 6-x-x^2$  
\onslide<2->{\[y = -x^2 - x + 6\]}
\begin{minipage}{0.55\textwidth}
\onslide<3->{
\begin{tikzpicture}[scale=0.8]
\begin{axis}[
xmin = -4, xmax = 3,
ymin = -4, ymax = 7,
xtick = {-3,-2,...,2},
ytick = {-3,-2,...,6}
]
\addplot[color=blue, very thick, samples=200, smooth] {-x^2-x+6};
\addplot[color=blue, mark=*] coordinates {(-0.5,6.25)};
\end{axis}
\end{tikzpicture}}
\end{minipage}
\begin{minipage}{0.4\textwidth}
\onslide<4->{Vertex: $\left(-\frac{1}{2},\frac{25}{4}\right)$} \\[12pt]
\onslide<5->{$a = -1$} \\[12pt]
\onslide<6->{$y = -\left(x+\frac{1}{2}\right)^2 + \frac{25}{4}$}
\end{minipage}
\end{frame}

\begin{frame}{Converting From Standard to General Form}
To convert from \newline
\[ y = a(x-h)^2 + k \]	\newline
form to 	\newline
\[ y = ax^2 + bx + c\]	\newline
just {\color{blue}\textbf{do the math}} and remember your \underline{order of operations}.
\end{frame}

\begin{frame}{Example 3}
(a) \quad Convert $y = (x+2)^2 - 3$ to general form.
\begin{align*}
	\onslide<2->{y &= (x+2)^2 - 3} \\[8pt]
    \onslide<3->{y &= x^2 + 4x + 4 - 3} \\[8pt]
    \onslide<4->{y &= x^2 + 4x + 1}	\\[8pt]
    \onslide<5->{y &= x^2 + 4x + 1}
\end{align*}
\end{frame}

\begin{frame}{Example 3}
(b) \quad Convert $y = -(x-7)^2 + 10$ to general form.
\begin{align*}
	\onslide<2->{y &= -(x-7)^2 + 10} \\[8pt]
	\onslide<3->{y &= -(x^2-14x+49) + 10} \\[8pt]
	\onslide<4->{y &= -x^2 + 14x - 49 + 10} \\[8pt]
	\onslide<5->{y &= -x^2 + 14x - 48}
\end{align*}
\end{frame}

\end{document}
